tests/lean/mk_constructor_fresh_names.lean
@@ -1,0 +1,24 @@
+open tactic
+
+example (fst fst_1 : nat) : fst = fst :=
+by do
+  ns ← mk_constructors_fresh_names `prod,
+  trace ns, -- [[fst_2, snd]]
+  constructor
+
+example (a : nat) : a = a :=
+by do
+  ns ← mk_constructors_fresh_names `acc,
+  trace ns, -- [[x, a_1]
+  constructor
+
+inductive Foo
+| mk₁ (a b c : nat)  : Foo
+| mk₂ (d e : bool)   : Foo
+| mk₃ (f g : Foo)    : Foo
+
+example (a d d_1 e : bool) : a = a :=
+by do
+  ns ← mk_constructors_fresh_names `Foo,
+  trace ns, -- [[a_1, b, c], [d_2, e_1], [f, g]]
+  constructor
